---
layout: directory
title: Ф-лы сокр. умножения
---

#### Формулы сокращенного умножения

$(a + b)^2 = a^2 + 2ab + b^2$

$(a - b)^2 = a^2 - 2ab + b^2$

$a^2 - b^2 = (a - b)(a + b)$

[Замените звёздочку](https://igorlsemenov.ru/math/алгебра/7/ф-лы_сокр._умножения/1)

[Сравните](https://igorlsemenov.ru/math/алгебра/7/ф-лы_сокр._умножения/2)

[Вычислите в уме](https://igorlsemenov.ru/math/алгебра/7/ф-лы_сокр._умножения/4)

[Замените звёздочки](https://igorlsemenov.ru/math/алгебра/7/ф-лы_сокр._умножения/5)

--- ---

$(a + b)^3 = a^3 + 3a^2b + 3ab^2 + b^3$

$(a - b)^3 = a^3 - 3a^2b + 3ab^2 - b^3$

--- ---

$a^3 + b^3 = (a + b)(a^2 - ab + b^2)$

$a^3 - b^3 = (a - b)(a^2 + ab + b^2)$
